formal-proofs/theories/lib/concurrent_linked_list/infinite_array/array_impl.v
@@ -1,0 +1,502 @@
+From iris.heap_lang Require Export proofmode notation lang.
+Require Import SegmentQueue.lib.concurrent_linked_list.segment_interfaces.
+
+Section SQSegment_impl.
+
+Variable maxSlots: positive.
+Variable pointerShift: positive.
+
+Definition newSegment: val :=
+  λ: "id" "prev" "pointers",
+  ref ("id", ref ("pointers" ≪ #(Zpos pointerShift)), ref "prev", ref NONE,
+       AllocN #(Zpos maxSlots) NONE).
+
+Definition getPrevLoc: val :=
+  λ: "this", Snd (Fst (Fst (!"this"))).
+
+Definition getNextLoc: val :=
+  λ: "this", Snd (Fst (!"this")).
+
+Definition getCleanedAndPointersLoc: val :=
+  λ: "this", Snd (Fst (Fst (Fst (!"this")))).
+
+Definition getId: val :=
+  λ: "this", Fst (Fst (Fst (Fst (!"this")))).
+
+Definition SQSegmentListNode :=
+  {| segment_interfaces.getPrevLoc := getPrevLoc;
+     segment_interfaces.getNextLoc := getNextLoc;
+  |}.
+
+Definition SQSegment :=
+  {| segment_interfaces.base := SQSegmentListNode;
+     segment_interfaces.newSegment := newSegment;
+     segment_interfaces.getId := getId;
+     segment_interfaces.maxSlots := Pos.to_nat maxSlots;
+     segment_interfaces.pointerShift := Pos.to_nat pointerShift;
+     segment_interfaces.getCleanedAndPointersLoc := getCleanedAndPointersLoc
+  |}.
+
+End SQSegment_impl.
+
+From iris.base_logic Require Import lib.invariants.
+From iris.algebra Require Import cmra auth list agree csum excl gset frac.
+Require Import SegmentQueue.lib.concurrent_linked_list.segment_spec.
+Require Import SegmentQueue.util.everything.
+
+Section infinite_array_segment_proof.
+
+Context `{heapG Σ}.
+
+Variable segment_size: positive.
+Variable pointer_shift: positive.
+Variable pointer_shift_bound:
+  Pos.to_nat segment_size < 2 ^ Pos.to_nat pointer_shift.
+
+Notation cell_algebra := (csumR (agreeR unitO) (* cell is cancelled *)
+                                (exclR unitO)) (* cancellation permit exists *).
+
+Record immutableValues :=
+  ImmutableValues {
+      segmentId: nat;
+      segmentNextLocation: loc;
+      segmentPrevLocation: loc;
+      segmentCleanedAndPointersLocation: loc;
+      segmentDataLocation: loc;
+    }.
+
+Inductive cellState := cellAlive
+                     | cellCancelled.
+
+Canonical Structure immutableValuesO := leibnizO immutableValues.
+
+Notation segment_algebra :=
+  (prodR
+     (authUR (listUR (optionUR cell_algebra))) (* Cells *)
+     (optionUR (agreeR immutableValuesO) (* Immutable contents of the segment *)
+  )).
+
+Class iSegmentG Σ := ISegmentG { iarray_inG :> inG Σ segment_algebra }.
+Definition iSegmentΣ : gFunctors := #[GFunctor segment_algebra].
+Instance subG_iSegmentΣ : subG iSegmentΣ Σ -> iSegmentG Σ.
+Proof. solve_inG. Qed.
+Context `{iSegmentG Σ}.
+
+Notation iProp := (iProp Σ).
+
+Let segment_size_nat := Pos.to_nat segment_size.
+
+Definition cell_algebra_from_state (state: cellState): cell_algebra :=
+  if state then Cinr (Excl ()) else Cinl (to_agree ()).
+
+Definition algebra_from_list
+           (values: immutableValues)
+           (state: list cellState): segment_algebra :=
+  (● ((fun (v: cellState) => Some (cell_algebra_from_state v)) <$> state),
+   Some (to_agree values)).
+
+Definition cell_is_cancelled γ id :=
+  own γ (◯ {[ id := Some (cell_algebra_from_state cellCancelled) ]}, ε).
+
+Global Instance cell_is_cancelled_persistent γ id:
+  Persistent (cell_is_cancelled γ id).
+Proof. apply _. Qed.
+
+Definition cell_cancellation_handle γ id :=
+  own γ (◯ {[ id := Some (cell_algebra_from_state cellAlive) ]}, ε).
+
+Theorem cell_cancellation_handle_exclusize γ id:
+  cell_cancellation_handle γ id -∗ cell_cancellation_handle γ id -∗ False.
+Proof.
+  iIntros "H1 H2".
+  iDestruct (own_valid_2 with "H1 H2") as %HValid. exfalso. move: HValid.
+  rewrite -pair_op. case=> /=.
+  rewrite -auth_frag_op auth_frag_valid list_singletonM_op list_singletonM_valid//.
+Qed.
+
+Theorem cell_with_handle_not_cancelled γ id:
+  cell_is_cancelled γ id -∗ cell_cancellation_handle γ id -∗ False.
+  iIntros "H1 H2".
+  iDestruct (own_valid_2 with "H1 H2") as %HValid. exfalso. move: HValid.
+  rewrite -pair_op. case=> /=.
+  rewrite -auth_frag_op auth_frag_valid list_singletonM_op list_singletonM_valid//.
+Qed.
+
+Lemma auth_cancel_cell values state γ id:
+  cell_cancellation_handle γ id -∗
+  own γ (algebra_from_list values state) ==∗
+  own γ (algebra_from_list values (<[ id := cellCancelled ]> state)) ∗
+  cell_is_cancelled γ id.
+Proof.
+  iIntros "HHandle Hγ".
+  iMod (own_update_2 with "Hγ HHandle") as "[$ $]"; last done.
+  apply prod_update; simpl; last done.
+  apply auth_update, list_lookup_local_update=> i.
+  rewrite list_fmap_insert.
+  destruct (lt_eq_lt_dec i id) as [[HLt| ->]|HGt].
+  - rewrite !list_lookup_singletonM_lt; try lia.
+    rewrite list_lookup_insert_ne //; last lia.
+  - rewrite !list_lookup_singletonM list_lookup_fmap.
+    destruct (decide (id < length state)%nat) as [HLt|HGe].
+    * rewrite list_lookup_insert; last by rewrite fmap_length.
+      apply lookup_lt_is_Some in HLt.
+      destruct HLt as [x ->]. simpl.
+      apply option_local_update, option_local_update.
+      rewrite /cell_algebra_from_state.
+      destruct x.
+      + apply replace_local_update; [apply _|done].
+      + apply local_update_valid. intros _ _.
+        case; first by intros HContra; inversion HContra.
+        rewrite csum_included.
+        case; first done.
+        by case; intros (? & ? & ? & ? & ?).
+    * apply local_update_valid.
+      intros _ _.
+      rewrite !lookup_ge_None_2; last lia.
+      2: by rewrite insert_length fmap_length; lia.
+      simpl.
+      case; first by intros HContra; inversion HContra.
+      intros HContra. by apply included_None in HContra.
+  - rewrite !list_lookup_singletonM_gt; try lia.
+    rewrite list_lookup_insert_ne //; last lia.
+Qed.
+
+Instance uniqueValue_fmap E: FMap (@uniqueValue Σ E).
+Proof.
+  intros A B f HUnique.
+  eapply UniqueValue with
+      (has_value := (fun γ v => ∃ v', has_value HUnique γ v' ∗ ⌜f v' = v⌝)%I);
+    try apply _.
+  iIntros (γ value1 value2) "H1 H2".
+  iDestruct "H1" as (values1) "[H1 %]".
+  iDestruct "H2" as (values2) "[H2 %]".
+  iDestruct (has_value_agrees with "H1 H2") as "<-".
+  by simplify_eq.
+Defined.
+
+Theorem immutableValues_uniqueValue: @uniqueValue Σ gname immutableValues.
+Proof.
+  eapply UniqueValue with
+      (has_value := (fun γ values => own γ (ε, Some (to_agree values)))%I);
+    try apply _.
+  iIntros (γ v1 v2) "H1 H2".
+  iDestruct (own_valid_2 with "H1 H2") as %[_ HValid]%pair_valid.
+  iPureIntro. move: HValid; simpl. rewrite -Some_op Some_valid.
+  intros HAgree. apply agree_op_invL' in HAgree. by inversion HAgree.
+Defined.
+
+Definition prev_uniqueValue :=
+  segmentPrevLocation <$> immutableValues_uniqueValue.
+
+Definition next_uniqueValue :=
+  segmentNextLocation <$> immutableValues_uniqueValue.
+
+Definition cleanedAndPointers_uniqueValue :=
+  segmentCleanedAndPointersLocation <$> immutableValues_uniqueValue.
+
+Definition id_uniqueValue :=
+  segmentId <$> immutableValues_uniqueValue.
+
+Definition dataLocation_uniqueValue :=
+  segmentDataLocation <$> immutableValues_uniqueValue.
+
+Variable (cell_is_owned: nat -> iProp).
+
+Definition segment_invariant (γ: gname) (values: immutableValues): iProp :=
+  [∗ list] i ∈ seq 0 segment_size_nat,
+  (cell_is_owned (segmentId values * segment_size_nat + i) ∨
+   (segmentDataLocation values +ₗ i) ↦ NONEV ∗ cell_cancellation_handle γ i)%I.
+
+Variable (N: namespace).
+
+Definition is_node γ (node: val): iProp :=
+  ∃ (ℓ: loc), ⌜node = #ℓ⌝ ∧
+              ∃ (values: immutableValues),
+                inv N (segment_invariant γ values) ∗
+                own γ (ε, Some (to_agree values)) ∗
+                inv_heap_inv ∗
+                ℓ ↦□ (fun v => v = (#(segmentId values),
+                                    #(segmentCleanedAndPointersLocation values),
+                                    #(segmentPrevLocation values),
+                                    #(segmentNextLocation values),
+                                    #(segmentDataLocation values))%V).
+
+Global Instance is_node_persistent γ node: Persistent (is_node γ node).
+Proof. apply _. Qed.
+
+Theorem getPrevLoc_spec γ node:
+  {{{ is_node γ node }}}
+    getPrevLoc SQSegmentListNode node
+  {{{ pℓ, RET #pℓ; has_value prev_uniqueValue γ pℓ }}}.
+Proof.
+  iIntros (Φ) "#HNode HΦ".
+  iDestruct "HNode" as (ℓ -> values) "#(HInv & HValues & #HHeapInv & HLoc)".
+  wp_lam. wp_bind (! _)%E.
+  iMod (inv_mapsto_acc with "HHeapInv HLoc") as (?) "(-> & Hℓ & HℓRestore)";
+    first done.
+  wp_load. iMod ("HℓRestore" with "Hℓ") as "_". iModIntro. wp_pures.
+  iApply "HΦ". iExists _. by iFrame "HValues".
+Qed.
+
+Theorem getNextLoc_spec γ node:
+  {{{ is_node γ node }}}
+    getNextLoc SQSegmentListNode node
+  {{{ nℓ, RET #nℓ; has_value next_uniqueValue γ nℓ }}}.
+Proof.
+  iIntros (Φ) "#HNode HΦ".
+  iDestruct "HNode" as (ℓ -> values) "#(HInv & HValues & #HHeapInv & HLoc)".
+  wp_lam. wp_bind (! _)%E.
+  iMod (inv_mapsto_acc with "HHeapInv HLoc") as (?) "(-> & Hℓ & HℓRestore)";
+    first done.
+  wp_load. iMod ("HℓRestore" with "Hℓ") as "_". iModIntro. wp_pures.
+  iApply "HΦ". iExists _. by iFrame "HValues".
+Qed.
+
+Let impl := (SQSegment segment_size pointer_shift).
+
+Theorem getCleanedAndPointersLoc_spec γ node:
+  {{{ is_node γ node }}}
+    getCleanedAndPointersLoc impl node
+  {{{ cℓ, RET #cℓ; has_value cleanedAndPointers_uniqueValue γ cℓ }}}.
+Proof.
+  iIntros (Φ) "#HNode HΦ".
+  iDestruct "HNode" as (ℓ -> values) "#(HInv & HValues & #HHeapInv & HLoc)".
+  wp_lam. wp_bind (! _)%E.
+  iMod (inv_mapsto_acc with "HHeapInv HLoc") as (?) "(-> & Hℓ & HℓRestore)";
+    first done.
+  wp_load. iMod ("HℓRestore" with "Hℓ") as "_". iModIntro. wp_pures.
+  iApply "HΦ". iExists _. by iFrame "HValues".
+Qed.
+
+Theorem getId_spec γ node:
+  {{{ is_node γ node }}}
+    getId impl node
+  {{{ id, RET #id; has_value id_uniqueValue γ id }}}.
+Proof.
+  iIntros (Φ) "#HNode HΦ".
+  iDestruct "HNode" as (ℓ -> values) "#(HInv & HValues & #HHeapInv & HLoc)".
+  wp_lam. wp_bind (! _)%E.
+  iMod (inv_mapsto_acc with "HHeapInv HLoc") as (?) "(-> & Hℓ & HℓRestore)";
+    first done.
+  wp_load. iMod ("HℓRestore" with "Hℓ") as "_". iModIntro. wp_pures.
+  iApply "HΦ". iExists _. by iFrame "HValues".
+Qed.
+
+Theorem node_unboxed γ node:
+  is_node γ node -∗ ⌜val_is_unboxed node⌝.
+Proof. iIntros "#HNode". by iDestruct "HNode" as (ℓ ->) "_". Qed.
+
+Definition node_linkedListNode: linkedListNodeSpec Σ (base impl) :=
+  {| segment_spec.getPrevLoc_spec := getPrevLoc_spec;
+     segment_spec.getNextLoc_spec := getNextLoc_spec;
+     segment_spec.linkedListNode_unboxed := node_unboxed |}.
+
+Theorem node_induces_id γ γ' node id id':
+  has_value id_uniqueValue γ id -∗
+  has_value id_uniqueValue γ' id' -∗
+  is_node γ  node -∗
+  is_node γ' node ==∗
+  ⌜id = id'⌝.
+Proof.
+  iIntros "HId HId' HNode HNode'".
+  iDestruct "HNode" as (ℓ -> values) "#(HInv & HValues & #HHeapInv & HLoc)".
+  iDestruct "HNode'" as (ℓ' HEq values') "#(HInv' & HValues' & #HHeapInv' & HLoc')".
+  iDestruct "HId" as (?) "[HId <-]". iDestruct "HId'" as (?) "[HId' <-]".
+  iDestruct (has_value_agrees with "HId HValues") as "->".
+  iDestruct (has_value_agrees with "HId' HValues'") as "->".
+  iDestruct (own_valid_2 with "HLoc HLoc'") as %HH.
+  iPureIntro. move: HH.
+  simplify_eq.
+  rewrite -auth_frag_op auth_frag_valid.
+  rewrite gmap.singleton_op gmap.singleton_valid pair_valid.
+  case=>_/=HH.
+  apply (@agree_op_inv' (option val -d> PropO)) in HH.
+  specialize (HH (Some (#(segmentId values),
+                        #(segmentCleanedAndPointersLocation values),
+                        #(segmentPrevLocation values),
+                        #(segmentNextLocation values),
+                        #(segmentDataLocation values)))%V).
+  simpl in *. inversion HH as [HH1 _]. specialize (HH1 eq_refl).
+  destruct values; destruct values'; simpl in *. by simplify_eq.
+Qed.
+
+Instance cellStateDecidable (v v': cellState): Decision (v = v').
+Proof. case v; case v'; by constructor. Defined.
+
+Definition segment_content γ alive_slots: iProp :=
+  ∃ values state,
+    ⌜count_matching (fun v => v = cellAlive) state = alive_slots⌝ ∧
+    own γ (algebra_from_list values state).
+
+Theorem cancel_cell γ id alive_slots:
+  cell_cancellation_handle γ id -∗
+  segment_content γ alive_slots ==∗
+  cell_is_cancelled γ id ∗ ∃ alive_slots',
+      ⌜alive_slots = S alive_slots'⌝ ∧ segment_content γ alive_slots'.
+Proof.
+  iIntros "HHandle HContent". iDestruct "HContent" as (values state HCount) "Hγ".
+  iAssert (⌜state !! id = Some cellAlive⌝)%I as %HLookup.
+  {
+    rewrite /algebra_from_list.
+    iDestruct (own_valid_2 with "Hγ HHandle") as
+        %[[(seg & HLookup & HIncluded)%list_singletonM_included
+                                      _]%auth_both_valid _]%pair_valid.
+    iPureIntro.
+    rewrite map_lookup in HLookup.
+    destruct (state !! id) as [state'|] eqn:HLookup'; last done.
+    simpl in *. simplify_eq.
+    destruct state'; first done.
+    move: HIncluded=> /=. rewrite Some_included. case.
+      + intros HContra. inversion HContra.
+      + rewrite csum_included. case; first done.
+        case; by intros (? & ? & ? & ? & ?).
+  }
+  destruct alive_slots as [|alive_slots'].
+  { exfalso. move: HCount HLookup. clear. move: id.
+    induction state as [|x xs]; first done. simpl.
+    destruct x; simpl; first done. by case. }
+  iMod (auth_cancel_cell with "HHandle Hγ") as "[Hγ $]".
+  iExists alive_slots'. iSplitR; first done.
+  iExists _, _. iFrame "Hγ". iPureIntro.
+  rewrite list_insert_alter. erewrite count_matching_alter; last done.
+  rewrite HCount /=. lia.
+Qed.
+
+Theorem newSegment_spec (id: nat) (prev: val) (pointers: nat):
+  {{{ inv_heap_inv }}}
+    newSegment impl #id prev #pointers
+    {{{ γ node pℓ nℓ cℓ, RET node;
+        is_node γ node
+        ∗ segment_content γ (maxSlots impl)
+        ∗ has_value id_uniqueValue γ id
+        ∗ has_value cleanedAndPointers_uniqueValue γ cℓ
+        ∗ has_value prev_uniqueValue γ pℓ
+        ∗ has_value next_uniqueValue γ nℓ
+        ∗ pℓ ↦ prev ∗ nℓ ↦ NONEV ∗ cℓ ↦ #(pointers ≪ pointerShift impl)
+    }}}.
+Proof.
+  iIntros (Φ) "#HInv HΦ". wp_lam. wp_pures.
+  wp_alloc dℓ as "Hdℓ"; first lia. wp_alloc nℓ as "Hnℓ".
+  wp_alloc pℓ as "Hpℓ". wp_alloc cℓ as "Hcℓ".
+  rewrite -wp_fupd.
+  wp_alloc ℓ as "Hℓ".
+  pose values := {|
+      segmentId := id;
+      segmentNextLocation := nℓ;
+      segmentPrevLocation := pℓ;
+      segmentCleanedAndPointersLocation := cℓ;
+      segmentDataLocation := dℓ;
+    |}.
+  iMod (own_alloc (
+            algebra_from_list values (replicate segment_size_nat cellAlive) ⋅
+            (ε, Some (to_agree values)) ⋅
+            (◯ replicate segment_size_nat
+               (Some (cell_algebra_from_state cellAlive)), ε)))
+    as (γ) "[[H● #HValues] HCancellation]".
+  {
+    rewrite /algebra_from_list -!pair_op /= pair_valid.
+    split.
+    - apply auth_both_valid. rewrite fmap_replicate.
+      split; first done.
+      apply list_lookup_valid=> i.
+      destruct (_ !! i) eqn:E; last done.
+      apply lookup_replicate in E. by destruct E as [-> _].
+    - apply Some_valid. rewrite agree_idemp. done.
+  }
+  iApply "HΦ".
+  replace (Z.pos pointer_shift) with (Z.of_nat (pointerShift impl));
+    last by rewrite /impl /=; lia.
+  iFrame "Hpℓ Hnℓ Hcℓ".
+  iSplitL "Hℓ HCancellation Hdℓ"; last iSplitL "H●".
+  - iExists _. iSplitR; first done. iExists values.
+    iFrame "HInv HValues".
+    iMod (make_inv_mapsto with "HInv Hℓ") as "Hℓ'"; first done;
+      last iDestruct (inv_mapsto_own_inv with "Hℓ'") as "$"; first done.
+    iMod (inv_alloc N _ (segment_invariant γ values) with "[-]") as "$";
+      last done.
+    rewrite /segment_invariant /segment_size_nat Z2Nat.inj_pos /array.
+    iAssert ([∗ list] i ∈ seq 0 (Pos.to_nat segment_size),
+             cell_cancellation_handle γ i)%I
+      with "[HCancellation]" as "HCancellation".
+    {
+      rewrite /cell_cancellation_handle.
+      iClear "HInv HValues".
+      remember (Pos.to_nat segment_size) as n. clear.
+      remember (Some _) as state. clear.
+      replace (replicate _ _) with (replicate 0 ε ++ replicate n state);
+        last done.
+      remember 0 as start. clear.
+      iInduction n as [|n'] "IH" forall (start); first done.
+      simpl.
+      assert ((replicate start ε ++ state :: replicate n' state)
+                ≡ (replicate (S start) ε ++ replicate n' state) ⋅
+                {[ start := state ]}) as ->.
+      {
+        replace (S start) with (start + 1) by lia.
+        rewrite replicate_plus /= -app_assoc /=.
+        apply list_equiv_lookup=> i. rewrite list_lookup_op.
+        destruct (lt_eq_lt_dec i start) as [[HLt| ->]|HGt].
+        - rewrite list_lookup_singletonM_lt; last lia.
+          rewrite !lookup_app_l; try rewrite replicate_length //.
+          by rewrite lookup_replicate_2; last lia.
+        - rewrite list_lookup_singletonM.
+          rewrite !lookup_app_r; try rewrite replicate_length //.
+          rewrite Nat.sub_diag /=. rewrite -Some_op ucmra_unit_left_id //.
+        - rewrite list_lookup_singletonM_gt; last lia.
+          rewrite !lookup_app_r replicate_length; try lia.
+          rewrite ucmra_unit_right_id.
+          destruct (i - start) eqn:E; first lia. done.
+      }
+      rewrite auth_frag_op pair_op_1 own_op.
+      iDestruct "HCancellation" as "[HCancellation $]".
+      iApply ("IH" with "HCancellation").
+    }
+    assert (([∗ list] i ↦ v ∈ seq 0 (Pos.to_nat segment_size),
+             (dℓ +ₗ i) ↦ InjLV #())%I ≡
+            ([∗ list] i↦v ∈ replicate (Pos.to_nat segment_size) (InjLV #()),
+              (dℓ +ₗ i) ↦ v)%I) as <-.
+    {
+      apply big_opL_gen_proper_2. done. by apply _.
+      intros k.
+      destruct (seq _ _ !! k) eqn:E.
+      - apply lookup_seq in E. destruct E as [-> Hk].
+        by rewrite lookup_replicate_2; last lia.
+      - apply lookup_ge_None in E. rewrite seq_length in E.
+        rewrite lookup_ge_None_2 // replicate_length. lia.
+    }
+    iCombine "Hdℓ" "HCancellation" as "H".
+    rewrite -big_sepL_sep.
+    iApply (big_sepL_mono with "H").
+    intros ? ? HEq. apply lookup_seq in HEq. destruct HEq as [-> Hk].
+    iIntros "[Hdℓ HCancHandle]". iRight. iFrame.
+  - rewrite /segment_content. iExists values, _. iFrame "H●".
+    iPureIntro. rewrite /impl /segment_size_nat /=.
+    remember (Pos.to_nat _) as listLen. clear.
+    induction listLen; first done. rewrite /= IHlistLen //.
+  - repeat iSplitR; iExists _; iFrame "HValues"; done.
+Qed.
+
+Lemma max_slots_bound: (0 < maxSlots impl < 2 ^ pointerShift impl)%nat.
+Proof. rewrite /impl /=. split; first lia; last done. Qed.
+
+End infinite_array_segment_proof.
+
+Canonical Structure node_segment `{!heapG Σ}
+          (cell_is_owned: nat -> iProp Σ) (N: namespace)
+          {segment_size pointer_shift: positive}
+          (limit: Pos.to_nat segment_size < 2 ^ Pos.to_nat pointer_shift)
+          `{!iSegmentG Σ}: segmentSpec Σ (SQSegment segment_size pointer_shift) :=
+  {|
+  segment_spec.linkedListNode_base :=
+    node_linkedListNode segment_size pointer_shift cell_is_owned N;
+  segment_spec.getId_spec :=
+    getId_spec segment_size pointer_shift cell_is_owned N;
+  segment_spec.getCleanedAndPointersLoc_spec :=
+    getCleanedAndPointersLoc_spec segment_size pointer_shift cell_is_owned N;
+  segment_spec.newSegment_spec :=
+    newSegment_spec segment_size pointer_shift cell_is_owned N;
+  segment_spec.max_slots_bound :=
+    max_slots_bound segment_size pointer_shift limit;
+  segment_spec.node_induces_id :=
+    node_induces_id segment_size cell_is_owned N;
+  |}.
