formal-proofs/theories/lib/concurrent_linked_list/infinite_array/array_spec.v
@@ -1,0 +1,72 @@
+From iris.program_logic Require Import atomic.
+From iris.heap_lang Require Export proofmode notation lang.
+
+Record infiniteArraySpec Σ `{!heapG Σ} :=
+  InfiniteArraySpec {
+      newInfiniteArray: val;
+      cancelCell: val;
+      findCell: val;
+      derefCellPointer: val;
+      cutoffMoveForward: val;
+      cutoffGetPointer: val;
+      infinite_array_name: Type;
+      is_infinite_array (N: namespace) (γ: infinite_array_name)
+                        (cell_is_owned: nat → iProp Σ): iProp Σ;
+      is_infinite_array_persistent N γ co:
+        Persistent (is_infinite_array N γ co);
+      infinite_array_mapsto (γ: infinite_array_name) (i: nat) (ℓ: loc): iProp Σ;
+      infinite_array_mapsto_persistent γ i ℓ:
+        Persistent (infinite_array_mapsto γ i ℓ);
+      infinite_array_mapsto_agree γ i ℓ ℓ':
+        infinite_array_mapsto γ i ℓ -∗ infinite_array_mapsto γ i ℓ' -∗ ⌜ℓ = ℓ'⌝;
+      is_infinite_array_cell_pointer (γ: infinite_array_name) (p: val) (i: nat):
+          iProp Σ;
+      is_infinite_array_cell_pointer_persistent γ p i:
+        Persistent (is_infinite_array_cell_pointer γ p i);
+      is_infinite_array_cutoff
+        (γ: infinite_array_name) (v: val) (start_index: nat): iProp Σ;
+      cell_is_cancelled (γ: infinite_array_name) (i: nat): iProp Σ;
+      cell_is_cancelled_persistent γ i: Persistent (cell_is_cancelled γ i);
+      cell_cancellation_handle (γ: infinite_array_name) (i: nat): iProp Σ;
+      cell_cancellation_handle_exclusive γ i:
+        cell_cancellation_handle γ i -∗ cell_cancellation_handle γ i -∗ False;
+      cell_cancellation_handle_not_cancelled γ i:
+        cell_is_cancelled γ i -∗ cell_cancellation_handle γ i -∗ False;
+      acquire_cell N γ cell_is_owned i ℓ:
+        is_infinite_array N γ cell_is_owned -∗
+        infinite_array_mapsto γ i ℓ -∗
+        ∀ Φ, (cell_is_owned i ∨ ℓ ↦ NONEV ∗ cell_cancellation_handle γ i
+                                ={⊤∖↑N}=∗ cell_is_owned i ∗ Φ) ==∗ Φ;
+      cancelCell_spec N γ co p i:
+        is_infinite_array N γ co -∗
+        is_infinite_array_cell_pointer γ p i -∗
+        <<< cell_cancellation_handle γ i >>>
+            cancelCell p @ ⊤
+        <<< cell_is_cancelled γ i, RET #() >>>;
+      findCell_spec N γ co p (source_id id: nat):
+        {{{ is_infinite_array N γ co ∗
+            is_infinite_array_cell_pointer γ p source_id }}}
+        findCell p #id @ ⊤
+        {{{ p' id', RET p'; is_infinite_array_cell_pointer γ p' id'
+            ∗ (⌜source_id <= id <= id'⌝ ∨
+              ⌜source_id > id ∧ id' = source_id⌝)%nat
+            ∗ [∗ list] i ∈ seq id (id' - id), cell_is_cancelled γ i
+        }}};
+      derefCellPointer_spec γ (p: val) i:
+        {{{ is_infinite_array_cell_pointer γ p i }}}
+          derefCellPointer p
+        {{{ ℓ, RET #ℓ; infinite_array_mapsto γ i ℓ }}};
+      cutoffMoveForward_spec γ (p v: val) i:
+        is_infinite_array_cell_pointer γ p i -∗
+        <<< ∀ start_index, is_infinite_array_cutoff γ v start_index >>>
+          cutoffMoveForward v p @ ⊤
+        <<< ∃ (success: bool), if success
+            then is_infinite_array_cutoff γ v (max start_index i)
+            else ▷ is_infinite_array_cutoff γ v start_index ∗
+                cell_is_cancelled γ start_index, RET #success >>>;
+      cutoffGetPointer_spec γ (v: val):
+        ⊢ <<< ∀ start_index, is_infinite_array_cutoff γ v start_index >>>
+          cutoffGetPointer v @ ⊤
+        <<< ∃ (p: val), is_infinite_array_cutoff γ v start_index ∗
+                        is_infinite_array_cell_pointer γ p start_index, RET p >>>
+    }.
